Rewriting theorems for executable semantics

hol/p4Lib.sig
@@ -10,5 +10,6 @@ val get_clause_assums : thm -> term list
 val find_clause : thm -> string -> thm option
 val find_clause_e_red : string -> thm option
 val find_clause_stmt_red : string -> thm option
+val find_clause_frames_red : string -> thm option
 
 end
